{
    "@context": {
        "dct": "http://purl.org/dc/terms/",
        "owl": "http://www.w3.org/2002/07/owl#",
        "rdf": "http://www.w3.org/1999/02/22-rdf-syntax-ns#",
        "rdfa": "http://www.w3.org/ns/rdfa#",
        "rdfs": "http://www.w3.org/2000/01/rdf-schema#",
        "schema": "http://schema.org/",
        "xsd": "http://www.w3.org/2001/XMLSchema#",
        "skos": "http://www.w3.org/2004/02/skos/core#"
    },
    "@graph": [
        {
            "@id": "schema:description",
            "@type": "rdf:Property",
            "owl:equivalentProperty": {
                "@id": "dct:description"
            },
            "rdfs:comment": "A description of the item.",
            "rdfs:label": "description",
            "schema:domainIncludes": {
                "@id": "schema:Thing"
            },
            "schema:rangeIncludes": {
                "@id": "schema:Text"
            },
            "schema:sameAs": {
                "@id": "https://schema.org/description"
            }
        },
        {
            "@id": "schema:schemaVersion",
            "@type": "rdf:Property",
            "rdfs:comment": "Indicates (by URL or string) a particular version of a schema.",
            "rdfs:label": "schemaVersion",
            "schema:domainIncludes": {
                "@id": ""
            },
            "schema:rangeIncludes": [
                {
                    "@id": "schema:Text"
                },
                {
                    "@id": "schema:URL"
                }
            ],
            "schema:sameAs": {
                "@id": "https://schema.org/schemaVersion"
            }
        },
        {
            "@id": "schema:version",
            "@type": "rdf:Property",
            "rdfs:comment": "Indicates (by URL or string) a particular version of an instrument.",
            "rdfs:label": "version",
            "schema:domainIncludes": {
                "@id": ""
            },
            "schema:rangeIncludes": [
                {
                    "@id": "schema:Text"
                },
                {
                    "@id": "schema:URL"
                }
            ],
            "schema:sameAs": {
                "@id": "https://schema.org/version"
            }
        },
        {
            "@id": "skos:prefLabel",
            "@type": "rdf:Property",
            "rdfs:comment": "The long name of the instrument or item.",
            "rdfs:label": "prefLabel",
            "schema:domainIncludes": {
                "@id": ""
            },
            "schema:rangeIncludes": {
                "@id": "schema:Text"
            },
            "schema:sameAs": {
                "@id": "http://www.w3.org/2004/02/skos/core#prefLabel"
            }
        },
        {
            "@id": "skos:altLabel",
            "@type": "rdf:Property",
            "rdfs:comment": "The short name of the instrument or item.",
            "rdfs:label": "altLabel",
            "schema:domainIncludes": {
                "@id": ""
            },
            "schema:rangeIncludes": {
                "@id": "schema:Text"
            },
            "schema:sameAs": {
                "@id": "http://www.w3.org/2004/02/skos/core#altLabel"
            }
        },
        {
            "@id": "schema:question",
            "@type": "rdf:Property",
            "rdfs:comment": "The text displayed for the item.",
            "rdfs:label": "question",
            "schema:domainIncludes": {
                "@id": ""
            },
            "schema:rangeIncludes": {
                "@id": "schema:Text"
            },
            "schema:sameAs": {
                "@id": "https://schema.org/question"
            }
        },
        {
            "@id": "schema:givenName",
            "@type": "rdf:Property",
            "rdfs:comment": "Given name. In the U.S., the first name of a Person. This can be used along with familyName instead of the name property.",
            "rdfs:label": "givenName",
            "schema:domainIncludes": {
                "@id": "schema:Person"
            },
            "schema:rangeIncludes": {
                "@id": "schema:Text"
            },
            "schema:sameAs": {
                "@id": "https://schema.org/givenName"
            }
        },
        {
            "@id": "schema:birthPlace",
            "@type": "rdf:Property",
            "rdfs:comment": "The place where the person was born.",
            "rdfs:label": "birthPlace",
            "schema:domainIncludes": {
                "@id": "schema:Person"
            },
            "schema:rangeIncludes": {
                "@id": "schema:Place"
            },
            "schema:sameAs": {
                "@id": "https://schema.org/birthPlace"
            }
        },
        {
            "@id": "schema:birthDate",
            "@type": "rdf:Property",
            "rdfs:comment": "Date of birth.",
            "rdfs:label": "birthDate",
            "schema:domainIncludes": {
                "@id": "schema:Person"
            },
            "schema:rangeIncludes": {
                "@id": "schema:Date"
            },
            "schema:sameAs": {
                "@id": "https://schema.org/birthDate"
            }
        },
        {
            "@id": "schema:familyName",
            "@type": "rdf:Property",
            "rdfs:comment": "Family name. In the U.S., the last name of an Person. This can be used along with givenName instead of the name property.",
            "rdfs:label": "familyName",
            "schema:domainIncludes": {
                "@id": "schema:Person"
            },
            "schema:rangeIncludes": {
                "@id": "schema:Text"
            },
            "schema:sameAs": {
                "@id": "https://schema.org/familyName"
            }
        },
        {
            "@id": "schema:additionalName",
            "@type": "rdf:Property",
            "rdfs:comment": "An additional name for a Person, can be used for a middle name.",
            "rdfs:label": "additionalName",
            "schema:domainIncludes": {
                "@id": "schema:Person"
            },
            "schema:rangeIncludes": {
                "@id": "schema:Text"
            },
            "schema:sameAs": {
                "@id": "https://schema.org/additionalName"
            }
        },
        {
            "@id": "schema:gender",
            "@type": "rdf:Property",
            "rdfs:comment": "Gender of the person. While http://schema.org/Male and http://schema.org/Female may be used, text strings are also acceptable for people who do not identify as a binary gender.",
            "rdfs:label": "gender",
            "schema:domainIncludes": {
                "@id": "schema:Person"
            },
            "schema:rangeIncludes": [
                {
                    "@id": "schema:GenderType"
                },
                {
                    "@id": "schema:Text"
                }
            ],
            "schema:sameAs": {
                "@id": "https://schema.org/gender"
            }
        }
    ]
}
